Some adjustments for #190. Some work on last spfconc proof. #189

automat/CaseStudy/MediumSPF.thy
@@ -12,13 +12,16 @@ imports Medium
 
 begin
 
+default_sort countable
+
 (* ----------------------------------------------------------------------- *)
   section {* MediumSPF Definition for Verification *}
 (* ----------------------------------------------------------------------- *)
 
 text {* @{term MedSPF}: Lossy medium function for the Alternating Bit Protocol. *}
-definition MedSPF :: "bool stream \<Rightarrow> 'a medMessage tsyn SPF" where
-  "MedSPF ora \<equiv> Abs_ufun (tsynbMed ora)"
+lift_definition MedSPF :: "bool stream \<Rightarrow> 'a medMessage tsyn SPF" is
+  "\<lambda> ora. tsynbMed ora"
+  by simp
 
 text{* @{term oraFun}: Function to create ora streams with True at position n.*}
 definition oraFun :: "nat \<Rightarrow> bool stream set" where
@@ -33,7 +36,7 @@ lemma medspf_insert: "(MedSPF ora) \<rightleftharpoons> sb = (Abs_ufun (tsynbMed
   by (simp add: MedSPF_def)
 
 text{* The domain of @{term MedSPF}. *}
-lemma medspf_ufdom: "ufDom\<cdot>(MedSPF ora) = medInDom"
+lemma medspf_ufdom[simp]: "ufDom\<cdot>(MedSPF ora) = medInDom"
   apply (simp add: ufDom_def)
   apply (simp add: ubclDom_ubundle_def MedSPF_def tsynbMed_def)
   apply (subst rep_abs_cufun2)
@@ -42,9 +45,9 @@ lemma medspf_ufdom: "ufDom\<cdot>(MedSPF ora) = medInDom"
   by (meson medin_dom someI_ex)
 
 text{* The range of @{term MedSPF}. *}
-lemma medspf_ufran: "ufRan\<cdot>(MedSPF ora) = medOutDom"
+lemma medspf_ufran[simp]: "ufRan\<cdot>(MedSPF ora) = medOutDom"
   apply (simp add: ufran_least)
-  apply (simp add: ubclLeast_ubundle_def medspf_ufdom ubclDom_ubundle_def)
+  apply (simp add: ubclLeast_ubundle_def ubclDom_ubundle_def)
   by (simp add: MedSPF_def tsynbmed_insert tsynbmed_ubundle_ubdom)
 
 text{* The domain of the output bundle of @{term MedSPF}. *}
@@ -85,7 +88,7 @@ lemma orafun_nempty: "oraFun n \<noteq> {}"
     using insert_not_empty ora_def by simp
   have sdrop_empty: "sdrop n\<cdot>(n\<star>\<up>False) = \<bottom>"
     by (simp add: sdropostake sntimes_stake)
-  then have sdrop_empty: "sdrop n\<cdot>ora = \<up>True\<infinity>"
+  then have sdrop_inf: "sdrop n\<cdot>ora = \<up>True\<infinity>"
     by (simp add: ora_def sdropl6)
   then have snth_true: "snth n ora"
     by (simp add: snth_def)
@@ -101,25 +104,95 @@ lemma orafun_nempty: "oraFun n \<noteq> {}"
     by blast
   qed
 
+lemma assumes "ora \<in> oraFun 0" shows "\<exists> ora1 n. ((ora = \<up>True \<bullet> ora1) \<and> ora1 \<in> oraFun n)"
+  proof -
+    obtain ora where ora_def: "\<exists> n. ora  = \<up>True \<bullet> ((n \<star> \<up>False) \<bullet> ((\<up>True)\<infinity>))"
+      by blast
+    obtain n where n_def: "ora  = \<up>True \<bullet> ((n \<star> \<up>False) \<bullet> ((\<up>True)\<infinity>))"
+      using ora_def by blast
+    have ora_shd_t: "shd ora  = True"
+      using ora_def shd1 by blast
+    have ora_fair: "#({True} \<ominus> ora) = \<infinity>"
+      using ora_def strict_slen by auto
+    then have "ora \<in> oraFun 0"
+      by (simp add: ora_shd_t oraFun_def)
+    obtain ora1 where ora1_def: "ora = \<up>True \<bullet> ora1"
+      using ora_def by blast
+    have ora1_stream: "ora1 = (n \<star> \<up>False) \<bullet> ((\<up>True)\<infinity>)"
+      using inject_scons n_def ora1_def by blast
+    have ora1_fair: "#({True} \<ominus> ora1) = \<infinity>"
+      using ora1_def ora_fair by auto
+    then have sdrop_inf: "sdrop n\<cdot>ora1 = \<up>True\<infinity>"
+      by (simp add: ora1_stream sdropl6)
+    have snth_ora1_t: "snth n ora1"
+      using sdrop_inf snth_def by force
+    have sdrop_k: "\<And>k. k<n \<Longrightarrow> sdrop k\<cdot>(n\<star>\<up>False) = (n-k)\<star>\<up>False"
+      by (metis (no_types, lifting) add_diff_inverse_nat less_Suc_eq not_less_eq sdropl6 sdrops_sinf 
+        sntimes_len sntimes_stake stake_add)
+    then have snth_ora1_f: "\<forall>k<n. \<not> snth k ora1"
+      by (metis less2nat linorder_not_le ora1_stream shd_sntime slen_snth_prefix snth_def sntimes_len 
+        zero_less_diff)
+    then have "ora1 \<in> oraFun n"
+      by (simp add: snth_ora1_f ora1_fair oraFun_def snth_ora1_t)
+    show ?thesis
+      apply (rule_tac x="ora1" in exI)
+      apply (rule_tac x="n" in exI)
+      apply (simp add: oraFun_def snth_ora1_f snth_ora1_t ora1_fair)
+  oops
+
+(* move to streams *)
+lemma sdrop_conc_geq:
+  "#x \<ge> Fin k \<Longrightarrow> sdrop k\<cdot>(x \<bullet> y) = (sdrop k\<cdot>x) \<bullet> y"
+apply (simp add: atomize_imp)
+apply (rule_tac x="x" in spec)
+apply (rule_tac x="y" in spec)
+apply (induct_tac k, auto)
+by (rule_tac x="xa" in scases, auto)
+
+lemma orafun0_orafunn: assumes "ora \<in> oraFun 0" obtains n where "ora = \<up>True \<bullet> ora1 \<and> ora1 \<in> oraFun n"
+  using assms
+  proof -
+    obtain ora1 where ora1_def: "ora = \<up>True \<bullet> ora1"
+      by (metis (full_types) assms orafun_nbot orafun_snth snth_shd surj_scons)
+    have ora1_fair: "#({True} \<ominus> ora1) = \<infinity>"
+      using assms ora1_def oraFun_def by force
+    obtain ora2 where ora2_def: "ora2 = sdropwhile (\<lambda>x. \<not>x)\<cdot>ora1"
+      by simp
+    then obtain n where n_def: "snth n ora1 = shd ora2"
+      by (metis (no_types, lifting) Inf'_neq_0 ex_snth_in_sfilter_nempty ora1_fair sdropwhile_idem 
+        singleton_iff slen_empty_eq snth_shd stakewhileDropwhile stakewhile_f strict_sfilter 
+        surj_scons tdw)
+    have snth_ora1_t: "snth n ora1"
+      by (metis Inf'_neq_0 ora2_def n_def ex_snth_in_sfilter_nempty ora1_fair sconc_snd_empty 
+        sdropwhile_resup singleton_iff slen_empty_eq snth2sdom stakewhileDropwhile stakewhile_dom 
+        surj_scons)
+    have ora1_stream: "ora1 = (n \<star> \<up>False) \<bullet> ora2"
+      apply (simp add: ora2_def)
+      sorry
+    have sdrop_k: "\<forall>k<n. sdrop k\<cdot>(n\<star>\<up>False) = (n-k) \<star> \<up>False"
+      by (metis (no_types, lifting) add_diff_inverse_nat less_Suc_eq not_less_eq sdropl6 sdrops_sinf 
+        sntimes_len sntimes_stake stake_add)
+    then have sdrop_k_conc: "\<forall>k<n. sdrop k\<cdot>((n\<star>\<up>False) \<bullet> ora2) = ((n-k) \<star> \<up>False) \<bullet> ora2"
+      by (simp add: sdrop_conc_geq)
+    have snth_ora1_f: "\<forall>k<n. \<not> snth k ora1"
+      by (metis shd1 srcdups_shd2 srcdups_sntimes_prefix strict_srcdups zero_less_diff ora1_stream 
+        snth_def sdrop_k_conc)
+    then have ora1_orafun: "ora1 \<in> oraFun n"
+      by (simp add: ora1_fair oraFun_def snth_ora1_t)
+    show ?thesis
+      sorry
+  qed
+
 (* ----------------------------------------------------------------------- *)
 subsection {* MedSPF step lemmata *}
 (* ----------------------------------------------------------------------- *)
 
-(*lemma copied can be deleted *)
-lemma spfConcIn_step[simp]:
-  assumes  "ubDom\<cdot>sb = ufDom\<cdot>spf"
-  shows "(spfConcIn sb1\<cdot>spf) \<rightleftharpoons> sb = spf \<rightleftharpoons> (ubConcEq sb1\<cdot>sb)" 
-  by (simp_all add: assms spfConcIn_def ubclDom_ubundle_def Int_absorb1)
-(**)
-
 lemma medspf_spfconc_null: assumes "ora \<in> oraFun n"  
   shows "spfConcIn (medIn -)\<cdot>(MedSPF ora) = spfConcOut (medOut -)\<cdot>(MedSPF ora)"
-  apply (rule spf_eq)
-  apply (simp add: medspf_ufdom)+
-  apply (subst medspf_ubdom)
-  apply (simp add: medspf_ufdom)
-  apply (rule ub_eq)
-  apply (simp add: medspf_ubdom medspf_ufdom)+
+  apply (rule spf_eq, simp_all)
+  apply (subst medspf_ubdom, simp)
+  apply (rule ub_eq, simp_all)
+  apply (simp add: medspf_ubdom)+
   using assms
   by (simp add: medspf_insert usclConc_stream_def medOutDom_def tsynbmed_getch_out 
     medingetstream_ubconc_null orafun_nbot tsynmed_sconc_null tsynmap_sconc medout_null 
@@ -142,12 +215,10 @@ lemma medspf_spfconc_msg_nzero: assumes "ora1 \<in> oraFun (Suc n)" obtains ora2
     have ora2_orafun: "ora2 \<in> oraFun n"
       by (simp add: ora2_f ora2_fair ora2_snth oraFun_def)
     have "spfConcIn (medIn (Msg m))\<cdot>(MedSPF ora1) = spfConcOut (medOut -)\<cdot>(MedSPF ora2)"
-      apply (rule spf_eq)
-      apply (simp add: medspf_ufdom)+
-      apply (subst medspf_ubdom)
-      apply (simp add: medspf_ufdom)
-      apply (rule ub_eq)
-      apply (simp add: medspf_ubdom medspf_ufdom)+
+      apply (rule spf_eq, simp_all)
+      apply (subst medspf_ubdom, simp)
+      apply (rule ub_eq, simp)
+      apply (simp add: medspf_ubdom)+
       using assms
       by (simp add: medspf_insert usclConc_stream_def medOutDom_def tsynbmed_getch_out ora2def 
         medingetstream_ubconc_msg tsynmed_sconc_msg_f tsynmap_sconc_null medout_null)
@@ -155,24 +226,26 @@ lemma medspf_spfconc_msg_nzero: assumes "ora1 \<in> oraFun (Suc n)" obtains ora2
      using ora2_orafun that by simp
   qed           
 
-lemma medspf_spfconc_msg_zero: assumes "ora1 \<in> oraFun 0" obtains ora2 where "ora2 \<in> oraFun n"
+lemma medspf_spfconc_msg_zero: assumes "ora1 \<in> oraFun 0" obtains ora2 where "\<exists>n. ora2 \<in> oraFun n"
   and "spfConcIn (medIn (Msg m))\<cdot>(MedSPF ora1) = spfConcOut (medOut (Msg m))\<cdot>(MedSPF ora2)"
 (*TODO*)
   using assms
   proof -
-    obtain ora2 where ora2_def: "ora2 \<in> oraFun n"
+    obtain ora2 where ora2_def: "\<exists>n .ora2 \<in> oraFun n"
       by (meson orafun_nempty subsetI subset_empty)
     have ora1_shd_t: "shd ora1 = True"
       using assms orafun_snth snth_shd by blast
     obtain ora where ora_def: "ora1 = \<up>True \<bullet> ora"
       by (metis (full_types) assms ora1_shd_t orafun_nbot surj_scons)
+    obtain n where "ora1 = \<up>True \<bullet> ora \<and> ora \<in> oraFun n"
+      using assms orafun0_orafunn by blast 
+    have ora_fair: "#({True} \<ominus> ora) = \<infinity>"
+      using assms oraFun_def ora_def by auto
     have "spfConcIn (medIn (Msg m))\<cdot>(MedSPF ora1) = spfConcOut (medOut (Msg m))\<cdot>(MedSPF ora2)"
-      apply (rule spf_eq)
-      apply (simp add: medspf_ufdom)+
-      apply (subst medspf_ubdom)
-      apply (simp add: medspf_ufdom)
-      apply (rule ub_eq)
-      apply (simp add: medspf_ubdom medspf_ufdom)+
+      apply (rule spf_eq, simp_all)
+      apply (subst medspf_ubdom, simp)
+      apply (rule ub_eq, simp_all)
+      apply (simp add: medspf_ubdom)+
       using assms
       apply (simp add: medspf_insert usclConc_stream_def ora_def medOutDom_def tsynbmed_getch_out 
         medout_msg medingetstream_ubconc_msg tsynmed_sconc_msg_t tsynmap_sconc_msg)
